Separate proofs about sequential spec styles

src/OptimisticFS.v
@@ -1,41 +1,3 @@
-Require TreeSeq.
-Require Import Prog.
-Require Import CCL.
-Require Import OptimisticTranslator.
-Require Import Pred PredCrash Hashmap.
-
-(* TODO: move these sequential spec tools to separate file *)
-Definition prog_double A T (spec: A -> PredCrash.rawpred -> SeqSpec T) (p: prog T) :=
-  forall T' (rx: T -> prog T'),
-    Hoare.corr2 (fun hm donecond crashcond =>
-                   exists a F_,
-                     seq_pre (spec a F_ hm) *
-                     [[ sync_invariant F_ ]] *
-                     [[ forall r, Hoare.corr2
-                               (fun hm' donecond_rx crashcond_rx =>
-                                  seq_post (spec a F_ hm) hm' r *
-                                  [[ donecond_rx = donecond ]] *
-                                  [[ crashcond_rx = crashcond ]]) (rx r) ]] *
-                     [[ forall hm_crash,
-                          F_ * seq_crash (spec a F_ hm) hm_crash *
-                          [[ exists l, hashmap_subset l hm hm_crash ]] =p=>
-                        crashcond hm_crash ]])%pred
-                (Prog.Bind p rx).
-
-Notation "'SPEC' {< a1 .. an , 'PRE' : hm pre 'POST' : hm' post 'CRASH' : hm'c crash >} p" :=
-  (prog_double
-     (fun a1 => .. (fun an =>
-                   (fun F_ =>
-                      fun hm => {|
-                          seq_pre := sep_star F_ pre%pred;
-                          seq_post := fun hm' => post F_%pred;
-                          seq_crash := fun hm'c => crash%pred;
-                        |}
-                )) .. ) p)
-    (at level 0, p at level 60,
-     hm at level 0, hm' at level 0, hm'c at level 0,
-     a1 closed binder, an closed binder).
-
 Require Import Prog.
 Require Import Log.
 Require Import BFile.
@@ -79,10 +41,15 @@ Require Import DirTreePred.
 Require Import DirTreeNames.
 Require Import DirTreeInodes.
 Require Import DirTreeSafe.
+
+Require Import SeqSpecs.
 Require Import TreeSeq.
 Import TREESEQ.
 
-Lemma corr2_exists : forall T A spec (p: prog T),
+Require Import CCL.
+Require Import OptimisticCache OptimisticTranslator.
+
+Local Lemma corr2_exists : forall T A spec (p: prog T),
     (forall (a:A), Hoare.corr2 (fun hm done crash => spec hm done crash a) p) ->
     Hoare.corr2 (fun hm done crash => exists a, spec hm done crash a)%pred p.
 Proof.
@@ -92,20 +59,42 @@ Proof.
   eapply H; eauto.
 Qed.
 
-Definition file_getattr_ok : forall fsxp inum mscs,
-    SPEC {< '(ds, ts, pathname, Fm, Ftop, Ftree, f),
-          PRE:hm LOG.rep (FSXPLog fsxp) (SB.rep fsxp) (LOG.NoTxn ds) (MSLL mscs) hm *
-              [[ treeseq_in_ds Fm Ftop fsxp mscs ts ds ]] *
-              [[ (Ftree * pathname |-> File inum f)%pred  (dir2flatmem2 (TStree ts!!)) ]]
-                POST: hm' RET:^(mscs',r)
-                          LOG.rep (FSXPLog fsxp) (SB.rep fsxp) (LOG.NoTxn ds) (MSLL mscs') hm' *
-                      [[ r = BFILE.BFAttr f /\ MSAlloc mscs' = MSAlloc mscs ]]
-                        CRASH: hm'
-                                 LOG.idempred (FSXPLog fsxp) (SB.rep fsxp) ds hm'
-                               >} AFS.file_get_attr fsxp inum mscs.
-Proof.
-  unfold prog_double; simpl; intros.
-  do 2 (apply corr2_exists; intros).
+Section OptimisticFS.
 
-  hoare.
-Qed.
+  Context {St:StateTypes}.
+  Variable G:Protocol St.
+  Variable P:CacheParams St.
+
+  Definition file_get_attr fsxp inum mscs :=
+    translate P (AFS.file_get_attr fsxp inum mscs).
+
+  Definition translation_spec A T (spec: SeqSpec A T) (p: prog T) :=
+    forall tid wb, cprog_spec G tid (translate_spec P spec wb) (translate P p wb).
+
+  Ltac spec_reflect :=
+    unfold prog_spec; simpl;
+    repeat (intros; apply corr2_exists);
+    hoare.
+
+  Definition file_getattr_ok : forall fsxp inum mscs,
+      translation_spec
+        (SPEC {< '(ds, ts, pathname, Fm, Ftop, Ftree, f),
+               PRE:hm LOG.rep (FSXPLog fsxp) (SB.rep fsxp) (LOG.NoTxn ds) (MSLL mscs) hm *
+                   [[ treeseq_in_ds Fm Ftop fsxp mscs ts ds ]] *
+                   [[ (Ftree * pathname |-> File inum f)%pred  (dir2flatmem2 (TStree ts!!)) ]]
+                     POST: hm' RET:^(mscs',r)
+                               LOG.rep (FSXPLog fsxp) (SB.rep fsxp) (LOG.NoTxn ds) (MSLL mscs') hm' *
+                           [[ r = BFILE.BFAttr f /\ MSAlloc mscs' = MSAlloc mscs ]]
+                             CRASH: hm'
+                                      LOG.idempred (FSXPLog fsxp) (SB.rep fsxp) ds hm'
+                                    >})
+        (AFS.file_get_attr fsxp inum mscs).
+  Proof.
+    unfold translation_spec; intros.
+    apply translate_ok.
+    apply prog_quadruple_spec_equiv.
+    spec_reflect.
+    (* oh dear, the frame predicate has been lost *)
+  Abort.
+
+End OptimisticFS.
